tests/fv/js-equiv/constant-condition-right.js
@@ -1,0 +1,4 @@
+{
+  let result = "kept";
+  if (result !== "kept") throw 0;
+}
