tests/fv/js-equiv/optional-chain-left.js
@@ -1,0 +1,10 @@
+{
+  let called = false;
+  function get() {
+    if (called) throw 0;
+    called = true;
+    return null;
+  }
+  let result = get()?.p;
+  if (!called || result !== undefined) throw 0;
+}
