tests/fv/js-equiv/optional-chain-right.js
@@ -1,0 +1,14 @@
+{
+  let called = false;
+  function get() {
+    if (called) throw 0;
+    called = true;
+    return null;
+  }
+  let receiver = get();
+  let result =
+    receiver === null || receiver === undefined
+      ? undefined
+      : receiver.p;
+  if (!called || result !== undefined) throw 0;
+}
