formal/ITreeCoreRegression.v
@@ -1,0 +1,257 @@
+From Stdlib Require Import String List ZArith Floats.
+From ESMetaFV Require Import Fragment Domain ITreeExec ITreeCore Spec.
+
+Import ListNotations.
+Local Open Scope string_scope.
+
+Definition untraced_tree_test_ast : ast :=
+  ALex "IdentifierName" "x" nil nil nil.
+
+Definition untraced_tree_test_input :
+  String.string * cstr * ast * list host_cache_entry * (val * list val) :=
+  ("untraced", nil, untraced_tree_test_ast, nil, (VUndef, nil)).
+
+Example lexical_undefined_is_represented_exactly :
+  ast_lex_sdo
+    (ALex "NoSubstitutionTemplate" "\\1" nil nil
+      [("TV", LVUndef)])
+    "TV" = Some VUndef.
+Proof. reflexivity. Qed.
+
+Example production_exec_is_untraced : production_exec = exec_itree.
+Proof. reflexivity. Qed.
+
+(** The production Test262 tree must not consume fuel on diagnostic
+    function-entry/exit markers.  A caller can still request the separately
+    constructed traced tree through [tt_trace_func]. *)
+Example make_test_tree_uses_untraced_semantics :
+  tt_tree (make_test_tree untraced_tree_test_input) =
+    exec_itree TEST262_MODULE
+      (script_prog nil untraced_tree_test_ast nil).
+Proof. reflexivity. Qed.
+
+Example make_test_tree_retains_lazy_trace_projection target :
+  tt_trace_func (make_test_tree untraced_tree_test_input) target =
+    exec_itree_trace_func TEST262_MODULE
+      (script_prog nil untraced_tree_test_ast nil) target.
+Proof. reflexivity. Qed.
+
+Example string_to_bigint_host_query_dispatches :
+  host_cop_query CToBigInt (VStr nil) = Some (HQStrToBigInt nil).
+Proof. reflexivity. Qed.
+
+Example string_to_bigint_host_result_contract :
+  host_result_well_typed (HQStrToBigInt nil) (VBigInt 0%Z) = true /\
+  host_result_well_typed (HQStrToBigInt nil) VUndef = true /\
+  host_result_well_typed (HQStrToBigInt nil) (VStr nil) = false.
+Proof. repeat split; reflexivity. Qed.
+
+Example mathop_exact_equality :
+  host_query_eqb (HQMathOp MAtan2 [1%Z; 2%Z])
+                 (HQMathOp MAtan2 [1%Z; 2%Z]) = true /\
+  host_query_eqb (HQMathOp MAtan2 [1%Z; 2%Z])
+                 (HQMathOp MAtan [1%Z; 2%Z]) = false /\
+  host_query_eqb (HQMathOp MAtan2 [1%Z; 2%Z])
+                 (HQMathOp MAtan2 [2%Z; 1%Z]) = false.
+Proof. repeat split; reflexivity. Qed.
+
+Example mathop_exact_arity_and_types :
+  host_mathop_query MAtan [VMath 3%Z] = Some (HQMathOp MAtan [3%Z]) /\
+  host_mathop_query MAtan nil = None /\
+  host_mathop_query MAtan [VMath 3%Z; VMath 4%Z] = None /\
+  host_mathop_query MAtan2 [VMath 3%Z; VMath 4%Z] =
+    Some (HQMathOp MAtan2 [3%Z; 4%Z]) /\
+  host_mathop_query MAtan2 [VMath 3%Z] = None /\
+  host_mathop_query MAtan2 [VMath 3%Z; VBool true] = None /\
+  host_mathop_query MAcosh [VMath 3%Z] = None /\
+  host_mathop_query MAsinh [VMath 3%Z] = None /\
+  host_mathop_query MAtanh [VMath 3%Z] = None.
+Proof. repeat split; reflexivity. Qed.
+
+Example mathop_host_result_contract :
+  host_result_well_typed (HQMathOp MSqrt [4%Z]) (VMath 2%Z) = true /\
+  host_result_well_typed (HQMathOp MSqrt [4%Z]) (VBool true) = false.
+Proof. split; reflexivity. Qed.
+
+Example mathop_typed_cache_lookup_is_exact :
+  typed_host_cache_lookup
+    (HQMathOp MSqrt [4%Z])
+    [mkHostCacheEntry (HQMathOp MSqrt [4%Z]) (VMath 2%Z)] =
+      Some (VMath 2%Z) /\
+  typed_host_cache_lookup
+    (HQMathOp MSqrt [9%Z])
+    [mkHostCacheEntry (HQMathOp MSqrt [4%Z]) (VMath 2%Z)] = None /\
+  typed_host_cache_lookup
+    (HQMathOp MSqrt [4%Z])
+    [mkHostCacheEntry (HQMathOp MSqrt [4%Z]) (VBool true)] = None.
+Proof. repeat split; reflexivity. Qed.
+
+Example math_to_number_exact_boundary_stays_pure :
+  host_cop_query CToNumber (VMath 9007199254740992%Z) = None /\
+  host_cop_query CToApproxNumber (VMath (-9007199254740992)%Z) = None /\
+  eval_cop CToNumber (VMath 9007199254740992%Z) =
+    Some (VNumber (9007199254740992.0000)%float).
+Proof. repeat split; reflexivity. Qed.
+
+Example math_to_number_inexact_values_query_for_both_conversions :
+  host_cop_query CToNumber (VMath 9007199254740993%Z) =
+    Some (HQMathToNumber 9007199254740993%Z) /\
+  host_cop_query CToApproxNumber (VMath 9007199254740993%Z) =
+    Some (HQMathToNumber 9007199254740993%Z).
+Proof. split; reflexivity. Qed.
+
+Example math_to_number_query_equality_keeps_the_signed_key :
+  host_query_eqb (HQMathToNumber 9007199254740993%Z)
+                 (HQMathToNumber 9007199254740993%Z) = true /\
+  host_query_eqb (HQMathToNumber 9007199254740993%Z)
+                 (HQMathToNumber (-9007199254740993)%Z) = false.
+Proof. split; reflexivity. Qed.
+
+Example math_to_number_host_result_contract_accepts_only_number :
+  host_result_well_typed
+    (HQMathToNumber 9007199254740993%Z)
+    (VNumber (9007199254740992.0000)%float) = true /\
+  host_result_well_typed
+    (HQMathToNumber 9007199254740993%Z)
+    (VMath 9007199254740992%Z) = false.
+Proof. split; reflexivity. Qed.
+
+Example math_to_number_typed_cache_lookup_is_exact :
+  typed_host_cache_lookup
+    (HQMathToNumber 9007199254740993%Z)
+    [mkHostCacheEntry
+       (HQMathToNumber 9007199254740993%Z)
+       (VNumber (9007199254740992.0000)%float)] =
+      Some (VNumber (9007199254740992.0000)%float) /\
+  typed_host_cache_lookup
+    (HQMathToNumber (-9007199254740993)%Z)
+    [mkHostCacheEntry
+       (HQMathToNumber 9007199254740993%Z)
+       (VNumber (9007199254740992.0000)%float)] = None /\
+  typed_host_cache_lookup
+    (HQMathToNumber 9007199254740993%Z)
+    [mkHostCacheEntry
+       (HQMathToNumber 9007199254740993%Z)
+       (VMath 9007199254740992%Z)] = None.
+Proof. repeat split; reflexivity. Qed.
+
+Definition observable_ast_child : ast :=
+  ALex "Child" "x" nil nil nil.
+
+Definition observable_ast_root : ast :=
+  ASyn "Root" nil 0 0
+    [Some observable_ast_child] ["Child"] nil nil.
+
+Definition observable_other_ast_root : ast :=
+  ASyn "Root" nil 0 0
+    [Some (ALex "Child" "y" nil nil nil)] ["Child"] nil nil.
+
+Example observable_same_alias_pattern_passes :
+  observable_outcome_eqb
+    (VAst (AstRuntime 1) observable_ast_root nil,
+     [VAst (AstRuntime 1) observable_ast_root nil])
+    (VAst (AstExported 10) observable_ast_root nil,
+     [VAst (AstExported 10) observable_ast_root nil]) = true.
+Proof. vm_compute. reflexivity. Qed.
+
+Example observable_distinct_actual_refs_cannot_share_expected_ref :
+  observable_outcome_eqb
+    (VAst (AstRuntime 1) observable_ast_root nil,
+     [VAst (AstRuntime 2) observable_ast_root nil])
+    (VAst (AstExported 10) observable_ast_root nil,
+     [VAst (AstExported 10) observable_ast_root nil]) = false.
+Proof. vm_compute. reflexivity. Qed.
+
+Example observable_one_actual_ref_cannot_map_to_two_expected_refs :
+  observable_outcome_eqb
+    (VAst (AstRuntime 1) observable_ast_root nil,
+     [VAst (AstRuntime 1) observable_ast_root nil])
+    (VAst (AstExported 10) observable_ast_root nil,
+     [VAst (AstExported 11) observable_ast_root nil]) = false.
+Proof. vm_compute. reflexivity. Qed.
+
+Example observable_ast_identity_key_includes_cursor_path :
+  observable_outcome_eqb
+    (VAst (AstRuntime 1) observable_ast_root nil,
+     [VAst (AstRuntime 1) observable_ast_root [0]])
+    (VAst (AstExported 10) observable_ast_root nil,
+     [VAst (AstExported 11) observable_ast_root [0]]) = true.
+Proof. vm_compute. reflexivity. Qed.
+
+Example observable_focused_ast_payload_stays_structural :
+  observable_outcome_eqb
+    (VAst (AstRuntime 1) observable_ast_root [0], nil)
+    (VAst (AstExported 10) observable_other_ast_root [0], nil) = false.
+Proof. vm_compute. reflexivity. Qed.
+
+Example observable_nested_ast_alias_pattern_passes :
+  observable_outcome_eqb
+    (VClo "f"
+       [("captured", VAst (AstRuntime 1) observable_ast_root nil)],
+     [VAst (AstRuntime 1) observable_ast_root nil])
+    (VClo "f"
+       [("captured", VAst (AstExported 10) observable_ast_root nil)],
+     [VAst (AstExported 10) observable_ast_root nil]) = true.
+Proof. vm_compute. reflexivity. Qed.
+
+Example observable_nested_ast_aliases_share_the_outcome_bijection :
+  observable_outcome_eqb
+    (VClo "f"
+       [("captured", VAst (AstRuntime 1) observable_ast_root nil)],
+     [VAst (AstRuntime 1) observable_ast_root nil])
+    (VClo "f"
+       [("captured", VAst (AstExported 10) observable_ast_root nil)],
+    [VAst (AstExported 11) observable_ast_root nil]) = false.
+Proof. vm_compute. reflexivity. Qed.
+
+Example observable_closure_captures_ignore_map_iteration_order :
+  observable_outcome_eqb
+    (VClo "f" [("x", VBool true); ("y", VBool false)], nil)
+    (VClo "f" [("y", VBool false); ("x", VBool true)], nil) = true.
+Proof. vm_compute. reflexivity. Qed.
+
+Example observable_continuation_captures_ignore_map_iteration_order :
+  observable_outcome_eqb
+    (VCont "f" [("x", VBool true); ("y", VBool false)] (Some 7), nil)
+    (VCont "f" [("y", VBool false); ("x", VBool true)] (Some 7), nil) = true.
+Proof. vm_compute. reflexivity. Qed.
+
+Example observable_capture_duplicates_are_last_binding_wins :
+  observable_outcome_eqb
+    (VClo "f"
+       [("x", VBool false); ("unused", VBool false); ("x", VBool true)],
+     nil)
+    (VClo "f"
+       [("x", VBool false); ("x", VBool true); ("unused", VBool false)],
+     nil) = true.
+Proof. vm_compute. reflexivity. Qed.
+
+Example observable_reordered_nested_ast_capture_threads_aliases :
+  observable_outcome_eqb
+    (VClo "f"
+       [("plain", VBool true);
+        ("node", VAst (AstRuntime 1) observable_ast_root nil)],
+     [VAst (AstRuntime 1) observable_ast_root nil])
+    (VClo "f"
+       [("node", VAst (AstExported 10) observable_ast_root nil);
+        ("plain", VBool true)],
+     [VAst (AstExported 10) observable_ast_root nil]) = true.
+Proof. vm_compute. reflexivity. Qed.
+
+Example observable_capture_value_mismatch_fails :
+  observable_outcome_eqb
+    (VClo "f" [("x", VBool true); ("y", VBool false)], nil)
+    (VClo "f" [("y", VBool true); ("x", VBool true)], nil) = false.
+Proof. vm_compute. reflexivity. Qed.
+
+Example observable_capture_domain_mismatch_fails :
+  observable_outcome_eqb
+    (VClo "f" [("x", VBool true)], nil)
+    (VClo "f" [("x", VBool true); ("y", VBool false)], nil) = false.
+Proof. vm_compute. reflexivity. Qed.
+
+Example observable_continuation_frame_identity_remains_strict :
+  observable_outcome_eqb
+    (VCont "f" [("x", VBool true)] (Some 7), nil)
+    (VCont "f" [("x", VBool true)] (Some 8), nil) = false.
+Proof. vm_compute. reflexivity. Qed.
