formal/ITreeSmokeExtract.v
@@ -1,0 +1,184 @@
+(** Temporary small extraction smoke test for the executable ITree path. *)
+
+From Stdlib Require Import Extraction Floats.
+From Stdlib Require Import ExtrOcamlBasic ExtrOcamlNatInt ExtrOcamlZBigInt.
+From Stdlib Require Import ExtrOcamlNativeString ExtrOCamlFloats ExtrOCamlInt63.
+From CRIS Require Import ExtrOcamlCRIS.
+
+From ESMetaFV Require Import Fragment ITreeExec Programs.
+
+Import ListNotations.
+
+(** [ExtrOcamlNativeString] names the OCaml standard-library module
+    [String].  This extraction also contains stdpp's Rocq module named
+    [String], so unqualified references such as [String.get] become
+    accidentally self-referential inside the generated module.  Keep the
+    native representation, but qualify every runtime operation. *)
+Extract Inductive string => "string"
+  [ """"""
+    "(fun (c, s) -> Stdlib.String.make 1 c ^ s)" ]
+  "(fun f0 f1 s ->
+      let l = Stdlib.String.length s in
+      if l = 0 then f0 ()
+      else f1 (Stdlib.String.get s 0) (Stdlib.String.sub s 1 (l - 1)))".
+
+Extract Inlined Constant String.string_dec => "(=)".
+Extract Inlined Constant String.eqb => "(=)".
+Extract Inlined Constant String.append => "(^)".
+Extract Inlined Constant String.concat => "Stdlib.String.concat".
+Extract Inlined Constant String.prefix =>
+  "(fun s1 s2 ->
+      let l1 = Stdlib.String.length s1
+      and l2 = Stdlib.String.length s2 in
+      l1 <= l2 && Stdlib.String.sub s2 0 l1 = s1)".
+Extract Inlined Constant String.string_of_list_ascii =>
+  "(fun l ->
+      let a = Array.of_list l in
+      Stdlib.String.init (Array.length a) (fun i -> a.(i)))".
+Extract Inlined Constant String.list_ascii_of_string =>
+  "(fun s ->
+      List.init (Stdlib.String.length s) (fun i -> Stdlib.String.get s i))".
+Extract Inlined Constant String.string_of_list_byte =>
+  "(fun l ->
+      let a = Array.of_list l in
+      Stdlib.String.init (Array.length a) (fun i -> a.(i)))".
+Extract Inlined Constant String.list_byte_of_string =>
+  "(fun s ->
+      List.init (Stdlib.String.length s) (fun i -> Stdlib.String.get s i))".
+
+Definition number_math_smoke_expr : expr :=
+  EConvert CToNumber
+    (EBinary BAdd
+      (EConvert CToMath (ENumber (1.0000000000000000)%float))
+      (EConvert CToMath (ENumber (2.0000000000000000)%float))).
+
+Definition number_math_smoke_main : func :=
+  mkFunc true "main" nil (IReturn number_math_smoke_expr).
+
+Definition number_math_smoke_query : host_query :=
+  HQNumberMathOp NMAdd
+    (1.0000000000000000)%float (2.0000000000000000)%float.
+
+Definition number_math_smoke_prog : prog :=
+  mkProgFull [number_math_smoke_main] None None
+    [mkHostCacheEntry number_math_smoke_query
+      (VNumber (3.0000000000000000)%float)] nil nil.
+
+Definition number_math_missing_prog : prog :=
+  mkProgFull [number_math_smoke_main] None None nil nil nil.
+
+Definition number_math_wrong_type_prog : prog :=
+  mkProgFull [number_math_smoke_main] None None
+    [mkHostCacheEntry number_math_smoke_query (VMath 3)] nil nil.
+
+Definition smoke_tree := exec_itree "ESMetaFV-Smoke" sum_prog.
+Definition number_math_smoke_tree :=
+  exec_itree "ESMetaFV-NumberMathSmoke" number_math_smoke_prog.
+Definition number_math_missing_tree :=
+  exec_itree "ESMetaFV-NumberMathMissing" number_math_missing_prog.
+Definition number_math_wrong_type_tree :=
+  exec_itree "ESMetaFV-NumberMathWrongType" number_math_wrong_type_prog.
+Definition main_return_tree :=
+  exec_itree "ESMetaFV-MainReturnSmoke" main_return_prog.
+Definition captured_param_tree :=
+  exec_itree "ESMetaFV-CapturedParamSmoke" captured_param_prog.
+Definition print_tree := exec_itree "ESMetaFV-PrintSmoke" print2_prog.
+Definition cont_tree := exec_itree "ESMetaFV-ContSmoke" cont_prog.
+Definition stale_cont_tree :=
+  exec_itree "ESMetaFV-StaleContSmoke" stale_cont_prog.
+Definition poison_cont_tree :=
+  exec_itree "ESMetaFV-PoisonContSmoke" poison_cont_prog.
+Definition repeat_cont_tree :=
+  exec_itree "ESMetaFV-RepeatContSmoke" repeat_cont_prog.
+Definition named_ast_tree :=
+  exec_itree "ESMetaFV-NamedAstSmoke" named_ast_prog.
+Definition ast_parent_exists_tree :=
+  exec_itree "ESMetaFV-AstParentExistsSmoke" ast_parent_exists_prog.
+Definition number_to_math_tree :=
+  exec_itree "ESMetaFV-NumberToMathSmoke" number_to_math_prog.
+Definition host_tostr_tree :=
+  exec_itree "ESMetaFV-HostToStrSmoke" host_tostr_prog.
+Definition math_host_tree :=
+  exec_itree "ESMetaFV-MathHostSmoke" math_host_prog.
+Definition math_to_number_host_tree :=
+  exec_itree "ESMetaFV-MathToNumberHostSmoke" math_to_number_host_prog.
+Definition host_missing_tree :=
+  exec_itree "ESMetaFV-HostMissingSmoke" host_missing_prog.
+Definition host_wrong_type_tree :=
+  exec_itree "ESMetaFV-HostWrongTypeSmoke" host_wrong_type_prog.
+Definition host_parse_tree :=
+  exec_itree "ESMetaFV-HostParseSmoke" host_parse_prog.
+Definition initial_parse_priority_tree :=
+  exec_itree "ESMetaFV-InitialParsePrioritySmoke"
+    initial_parse_priority_prog.
+Definition host_parse_wrong_params_tree :=
+  exec_itree "ESMetaFV-HostParseWrongParamsSmoke"
+    host_parse_wrong_params_prog.
+Definition host_parse_failure_tree :=
+  exec_itree "ESMetaFV-HostParseFailureSmoke"
+    host_parse_failure_prog.
+Definition integer_keys_tree :=
+  exec_itree "ESMetaFV-IntegerKeysSmoke" integer_keys_prog.
+Definition duplicate_literals_tree :=
+  exec_itree "ESMetaFV-DuplicateLiteralsSmoke" duplicate_literals_prog.
+Definition initial_record_keys_tree :=
+  exec_itree "ESMetaFV-InitialRecordKeysSmoke" initial_record_keys_prog.
+Definition runtime_record_keys_tree :=
+  exec_itree "ESMetaFV-RuntimeRecordKeysSmoke" runtime_record_keys_prog.
+Definition runtime_empty_record_keys_tree :=
+  exec_itree "ESMetaFV-RuntimeEmptyRecordKeysSmoke"
+    runtime_empty_record_keys_prog.
+Definition runtime_singleton_record_keys_tree :=
+  exec_itree "ESMetaFV-RuntimeSingletonRecordKeysSmoke"
+    runtime_singleton_record_keys_prog.
+Definition copied_singleton_record_keys_tree :=
+  exec_itree "ESMetaFV-CopiedSingletonRecordKeysSmoke"
+    copied_singleton_record_keys_prog.
+Definition expanded_record_keys_tree :=
+  exec_itree "ESMetaFV-ExpandedRecordKeysSmoke" expanded_record_keys_prog.
+Definition assigned_record_keys_tree :=
+  exec_itree "ESMetaFV-AssignedRecordKeysSmoke" assigned_record_keys_prog.
+Definition copied_record_keys_tree :=
+  exec_itree "ESMetaFV-CopiedRecordKeysSmoke" copied_record_keys_prog.
+Definition record_refinement_tree :=
+  exec_itree "ESMetaFV-RecordRefinementSmoke" record_refinement_prog.
+Definition record_refinement_addr_tree :=
+  exec_itree "ESMetaFV-RecordRefinementAddrSmoke"
+    record_refinement_addr_prog.
+Definition completion_discriminant_tree :=
+  exec_itree "ESMetaFV-CompletionDiscriminantSmoke"
+    completion_discriminant_prog.
+Definition runtime_syn_tree :=
+  exec_itree "ESMetaFV-RuntimeSyntacticSmoke" runtime_syn_prog.
+Definition runtime_leaf_fresh_tree :=
+  exec_itree "ESMetaFV-RuntimeLeafFreshSmoke" runtime_leaf_fresh_prog.
+Definition number_int_refinement_tree :=
+  exec_itree "ESMetaFV-NumberIntRefinementSmoke"
+    number_int_refinement_prog.
+Definition number_nonneg_int_tree :=
+  exec_itree "ESMetaFV-NumberNonNegIntSmoke" number_nonneg_int_prog.
+Definition function_object_refinement_tree :=
+  exec_itree "ESMetaFV-FunctionObjectRefinementSmoke"
+    function_object_refinement_prog.
+
+Extraction "itree_smoke.ml"
+  smoke_tree
+  number_math_smoke_tree number_math_missing_tree number_math_wrong_type_tree
+  main_return_tree captured_param_tree print_tree cont_tree
+  stale_cont_tree poison_cont_tree repeat_cont_tree
+  named_ast_tree number_to_math_tree
+  ast_parent_exists_tree
+  host_tostr_tree math_host_tree math_to_number_host_tree
+  host_missing_tree host_wrong_type_tree
+  host_parse_tree initial_parse_priority_tree
+  host_parse_wrong_params_tree host_parse_failure_tree
+  integer_keys_tree duplicate_literals_tree
+  initial_record_keys_tree runtime_record_keys_tree
+  runtime_empty_record_keys_tree runtime_singleton_record_keys_tree
+  copied_singleton_record_keys_tree
+  expanded_record_keys_tree assigned_record_keys_tree copied_record_keys_tree
+  record_refinement_tree record_refinement_addr_tree
+  completion_discriminant_tree
+  runtime_syn_tree runtime_leaf_fresh_tree
+  number_int_refinement_tree number_nonneg_int_tree
+  function_object_refinement_tree.
